LibTactics.v
@@ -5192,3 +5192,26 @@ Ltac autorewrite_in_star_patch cont :=
   intro_until_mark.
 
 (* End of experimental features *)
+
+Tactic Notation "destructs" constr(E) :=
+  destruct ltac:(applys E).
+Tactic Notation "destructs" constr(E) "as" simple_intropattern(P) :=
+  destruct ltac:(applys E) as P.
+Tactic Notation "destructs" constr(E0) constr(A1) :=
+  destructs (>> E0 A1).
+Tactic Notation "destructs" constr(E0) constr(A1) "as" simple_intropattern(P) :=
+  destructs (>> E0 A1) as P.
+Tactic Notation "destructs" constr(E0) constr(A1) constr(A2) :=
+  destructs (>> E0 A1 A2).
+Tactic Notation "destructs" constr(E0) constr(A1) constr(A2) "as" simple_intropattern(P) :=
+  destructs (>> E0 A1 A2) as P.
+Tactic Notation "destructs" constr(E0) constr(A1) constr(A2) constr(A3) :=
+  destructs (>> E0 A1 A2 A3).
+Tactic Notation "destructs" constr(E0) constr(A1) constr(A2) constr(A3) "as" simple_intropattern(P) :=
+  destructs (>> E0 A1 A2 A3) as P.
+Tactic Notation "destructs" constr(E0) constr(A1) constr(A2) constr(A3) constr(A4) "as" simple_intropattern(P) :=
+  destructs (>> E0 A1 A2 A3 A4) as P.
+Tactic Notation "destructs" constr(E0) constr(A1) constr(A2) constr(A3) constr(A4) constr(A5) "as" simple_intropattern(P) :=
+  destructs (>> E0 A1 A2 A3 A4 A5) as P.
+Tactic Notation "destructs" constr(E0) constr(A1) constr(A2) constr(A3) constr(A4) constr(A5) constr(A6) "as" simple_intropattern(P) :=
+  destructs (>> E0 A1 A2 A3 A4 A5 A6) as P.
